changed call history to be part of stack frame

evaluation.lean
@@ -1,16 +1,16 @@
 import .syntax .notations
 
 def unop.apply: unop → value → option value
-| unop.not value.true                  := value.false
-| unop.not value.false                 := value.true
-| unop.isInt (value.num _)             := value.true
-| unop.isInt _                         := value.false
-| unop.isBool value.true               := value.true
-| unop.isBool value.false              := value.true
-| unop.isBool _                        := value.false
-| unop.isFunc (value.func _ _ _ _ _ _) := value.true
-| unop.isFunc _                        := value.false
-| _ _                                  := none
+| unop.not value.true                    := value.false
+| unop.not value.false                   := value.true
+| unop.isInt (value.num _)               := value.true
+| unop.isInt _                           := value.false
+| unop.isBool value.true                 := value.true
+| unop.isBool value.false                := value.true
+| unop.isBool _                          := value.false
+| unop.isFunc (value.func _ _ _ _ _ _ _) := value.true
+| unop.isFunc _                          := value.false
+| _ _                                    := none
 
 noncomputable def binop.apply: binop → value → value → option value
 | binop.plus (value.num n₁) (value.num n₂)  := value.num (n₁ + n₂)
@@ -32,63 +32,63 @@ noncomputable def binop.apply: binop → value → value → option value
 | _ _ _                                     := none
 
 
-inductive step : stack → historyitem → stack → Prop
-notation s₁ `⟶` c `,` s₂:100 := step s₁ c s₂
+inductive step : stack → stack → Prop
+notation s₁ `⟶` s₂:100 := step s₁ s₂
 
-| ctx {s s': stack} {c: historyitem} {σ: env} {y f x: var} {e: exp}:
-    (s ⟶ c, s') →
-    (s · [σ, let y = f[x] in e] ⟶ c, (s' · [σ, let y = f[x] in e]))
+| ctx {s s': stack} {H: history} {σ: env} {y f x: var} {e: exp}:
+    (s ⟶ s') →
+    (s · [H, σ, let y = f[x] in e] ⟶ (s' · [H, σ, let y = f[x] in e]))
 
-| tru {σ: env} {x: var} {e: exp}:
-    (σ, lett x = true in e) ⟶ nop, (σ[x↦value.true], e)
+| tru {H: history} {σ: env} {x: var} {e: exp}:
+    (H, σ, lett x = true in e) ⟶ (H, σ[x↦value.true], e)
 
-| fals {σ: env} {x: var} {e: exp}:
-    (σ, letf x = false in e) ⟶ nop, (σ[x↦value.false], e)
+| fals {H: history} {σ: env} {x: var} {e: exp}:
+    (H, σ, letf x = false in e) ⟶ (H, σ[x↦value.false], e)
 
-| num {σ: env} {x: var} {e: exp} {n: ℤ}:
-    (σ, letn x = n in e) ⟶ nop, (σ[x↦value.num n], e)
+| num {H: history} {σ: env} {x: var} {e: exp} {n: ℤ}:
+    (H, σ, letn x = n in e) ⟶ (H, σ[x↦value.num n], e)
 
-| closure {σ: env} {R S: spec} {f x: var} {e₁ e₂: exp}:
-    (σ, letf f[x] req R ens S {e₁} in e₂) ⟶ nop,
-    (σ[f↦value.func f x R S e₁ σ], e₂)
+| closure {H: history} {σ: env} {R S: spec} {f x: var} {e₁ e₂: exp}:
+    (H, σ, letf f[x] req R ens S {e₁} in e₂) ⟶ 
+    (H, σ[f↦value.func f x R S e₁ H σ], e₂)
 
-| unop {op: unop} {σ: env} {x y: var} {e: exp} {v₁ v: value}:
+| unop {H: history} {op: unop} {σ: env} {x y: var} {e: exp} {v₁ v: value}:
     (σ x = v₁) →
     (unop.apply op v₁ = v) →
-    ((σ, letop y = op [x] in e) ⟶ nop, (σ[y↦v], e))
+    ((H, σ, letop y = op [x] in e) ⟶ (H, σ[y↦v], e))
 
-| binop {op: binop} {σ: env} {x y z: var} {e: exp} {v₁ v₂ v: value}:
+| binop {H: history} {op: binop} {σ: env} {x y z: var} {e: exp} {v₁ v₂ v: value}:
     (σ x = v₁) →
     (σ y = v₂) →
     (binop.apply op v₁ v₂ = v) →
-    ((σ, letop2 z = op [x, y] in e) ⟶ nop, (σ[z↦v], e))
+    ((H, σ, letop2 z = op [x, y] in e) ⟶ (H, σ[z↦v], e))
 
-| app {σ σ': env} {R S: spec} {f g x y z: var} {e e': exp} {v: value}:
-    (σ f = value.func g z R S e σ') →
+| app {H H': history} {σ σ': env} {R S: spec} {f g x y z: var} {e e': exp} {v: value}:
+    (σ f = value.func g z R S e H' σ') →
     (σ x = v) →
-    ((σ, letapp y = f[x] in e') ⟶ nop,
-    ((σ'[g↦value.func g z R S e σ'][z↦v], e) · [σ, let y = f[x] in e']))
+    ((H, σ, letapp y = f[x] in e') ⟶
+    ((H', σ'[g↦value.func g z R S e H' σ'][z↦v], e) · [H, σ, let y = f[x] in e']))
 
-| return {σ₁ σ₂ σ₃: env} {f g gx x y z: var} {R S: spec} {e e': exp} {v vₓ: value}:
+| return {H₁ H₂ H₃: history} {σ₁ σ₂ σ₃: env} {f g gx x y z: var} {R S: spec} {e e': exp} {v vₓ: value}:
     (σ₁ z = v) →
-    (σ₂ f = value.func g gx R S e σ₃) →
+    (σ₂ f = value.func g gx R S e H₃ σ₃) →
     (σ₂ x = vₓ) →
-    ((σ₁, exp.return z) · [σ₂, let y = f[x] in e'] ⟶ call g gx R S e σ₃ vₓ, (σ₂[y↦v], e'))
+    ((H₁, σ₁, exp.return z) · [H₂, σ₂, let y = f[x] in e'] ⟶ (H₂ · call g gx R S e H₃ σ₃ vₓ, σ₂[y↦v], e'))
 
-| ite_true {σ: env} {e₁ e₂: exp} {x: var}:
+| ite_true {H: history} {σ: env} {e₁ e₂: exp} {x: var}:
     (σ x = value.true) →
-    ((σ, exp.ite x e₁ e₂) ⟶ nop, (σ, e₁))
+    ((H, σ, exp.ite x e₁ e₂) ⟶ (H, σ, e₁))
 
-| ite_false {σ: env} {e₁ e₂: exp} {x: var}:
+| ite_false {H: history} {σ: env} {e₁ e₂: exp} {x: var}:
     (σ x = value.false) →
-    ((σ, exp.ite x e₁ e₂) ⟶ nop, (σ, e₂))
+    ((H, σ, exp.ite x e₁ e₂) ⟶ (H, σ, e₂))
 
-notation s₁ `⟶` c `,` s₂:100 := step s₁ c s₂
+notation s₁ `⟶` s₂:100 := step s₁ s₂
 
 inductive trans_step : stack → stack → Prop
 notation s `⟶*` s':100 := trans_step s s'
-| rfl {s: stack}                                  : s ⟶* s
-| trans {s s' s'': stack} {c: historyitem} : (s ⟶ c, s') → (s' ⟶* s'') → (s ⟶* s'')
+| rfl {s: stack}          : s ⟶* s
+| trans {s s' s'': stack} : (s ⟶ s') → (s' ⟶* s'') → (s ⟶* s'')
 
 notation s `⟶*` s':100 := trans_step s s'
 
@@ -101,12 +101,12 @@ lemma binop.eq_of_equal_values {v: value}: binop.apply binop.eq v v = value.true
   show binop.apply binop.eq v v =  value.true, by simp[this]
 
 lemma unop.isFunc.inv {v: value}: unop.apply unop.isFunc v = value.true → 
-      ∃ (f x: var) (R S: spec) (e: exp) (σ: env), v = value.func f x R S e σ :=
+      ∃ (f x: var) (R S: spec) (e: exp) (H: history) (σ: env), v = value.func f x R S e H σ :=
   assume isFunc_is_true: unop.apply unop.isFunc v = value.true,
   begin
-    cases v with n f x R S e σ,
+    cases v with n f x R S e H σ,
 
-    show ∃ (f x: var) (R S: spec) (e: exp) (σ: env), value.true = value.func f x R S e σ, from (
+    show ∃ (f x: var) (R S: spec) (e: exp) (H: history) (σ: env), value.true = value.func f x R S e H σ, from (
       have h1: (unop.apply unop.isFunc value.true = value.true), from isFunc_is_true,
       have h2: (unop.apply unop.isFunc value.true = value.false), by unfold unop.apply,
       have some value.true = some value.false, from eq.trans h1.symm h2,
@@ -114,7 +114,7 @@ lemma unop.isFunc.inv {v: value}: unop.apply unop.isFunc v = value.true →
       false.elim (value._mut_.no_confusion this)
     ),
 
-    show ∃ (f x: var) (R S: spec) (e: exp) (σ: env), value.false = value.func f x R S e σ, from (
+    show ∃ (f x: var) (R S: spec) (e: exp) (H: history) (σ: env), value.false = value.func f x R S e H σ, from (
       have h1: (unop.apply unop.isFunc value.false = value.true), from isFunc_is_true,
       have h2: (unop.apply unop.isFunc value.false = value.false), by unfold unop.apply,
       have some value.true = some value.false, from eq.trans h1.symm h2,
@@ -122,7 +122,7 @@ lemma unop.isFunc.inv {v: value}: unop.apply unop.isFunc v = value.true →
       false.elim (value._mut_.no_confusion this)
     ),
 
-    show ∃ (f x: var) (R S: spec) (e: exp) (σ: env), value.num n = value.func f x R S e σ, from (
+    show ∃ (f x: var) (R S: spec) (e: exp) (H: history) (σ: env), value.num n = value.func f x R S e H σ, from (
       have h1: (unop.apply unop.isFunc (value.num n) = value.true), from isFunc_is_true,
       have h2: (unop.apply unop.isFunc (value.num n) = value.false), by unfold unop.apply,
       have some value.true = some value.false, from eq.trans h1.symm h2,
@@ -130,16 +130,17 @@ lemma unop.isFunc.inv {v: value}: unop.apply unop.isFunc v = value.true →
       false.elim (value._mut_.no_confusion this)
     ),
 
-    show ∃ (f_1 x_1: var) (R_1 S_1: spec) (e_1: exp) (σ_1: env),
-        value.func f x R S e σ = value.func f_1 x_1 R_1 S_1 e_1 σ_1, from (
-      exists.intro f (exists.intro x (exists.intro R (exists.intro S (exists.intro e (exists.intro σ rfl)))))
+    show ∃ (f_1 x_1: var) (R_1 S_1: spec) (e_1: exp) (H_1: history) (σ_1: env),
+        value.func f x R S e H σ = value.func f_1 x_1 R_1 S_1 e_1 H_1 σ_1, from (
+      exists.intro f (exists.intro x (exists.intro R (exists.intro S
+                     (exists.intro e (exists.intro H (exists.intro σ rfl))))))
     )
   end
 
 lemma unop.isBool.inv {v: value}: unop.apply unop.isBool v = value.true → (v = value.true) ∨ (v = value.false) :=
   assume isBool_is_true: unop.apply unop.isBool v = value.true,
   begin
-    cases v with n f x R S e σ,
+    cases v with n f x R S e H σ,
 
     show ((value.true = value.true) ∨ (value.true = value.false)), from (
       or.inl rfl
@@ -157,9 +158,9 @@ lemma unop.isBool.inv {v: value}: unop.apply unop.isBool v = value.true → (v =
       false.elim (value._mut_.no_confusion this)
     ),
 
-    show (value.func f x R S e σ = value.true ∨ (value.func f x R S e σ = value.false)), from (
-      have h1: unop.apply unop.isBool (value.func f x R S e σ) = ↑value.true, from isBool_is_true,
-      have h2: (unop.apply unop.isBool (value.func f x R S e σ) = value.false), by unfold unop.apply,
+    show (value.func f x R S e H σ = value.true ∨ (value.func f x R S e H σ = value.false)), from (
+      have h1: unop.apply unop.isBool (value.func f x R S e H σ) = ↑value.true, from isBool_is_true,
+      have h2: (unop.apply unop.isBool (value.func f x R S e H σ) = value.false), by unfold unop.apply,
       have some value.true = some value.false, from eq.trans h1.symm h2,
       have value.true = value.false, from option.some.inj this,
       false.elim (value._mut_.no_confusion this)
