freevars.lean
@@ -397,63 +397,54 @@ lemma free_in_vc.univ.same.inv {P: vc} {x: var}: ¬ free_in_vc x (vc.univ x P) :
     }
   end
 
-lemma call_history_closed (H: callhistory) (x: var): ¬ free_in_prop x (calls_to_prop H) :=
-  list.rec_on H
-  ( -- empty history
-    assume x_free: free_in_prop x (calls_to_prop list.nil),
-    have calls_to_prop list.nil = value.true, from rfl,
-    have x_free_in_true: free_in_prop x value.true, from this ▸ x_free,
-    show «false», by begin
-      cases x_free_in_true,
-      case free_in_prop.term x_free_in_term {
-        cases x_free_in_term
-      }
-    end
-  )
-  ( -- hist :: rest
-    assume h: historyitem,
-    assume rest: callhistory,
-    assume ih: ¬ free_in_prop x (calls_to_prop rest),
-    historyitem.cases_on h
-    ( -- <nop> :: rest
-      have h2: ¬ free_in_prop x (calls_to_prop rest), from ih,
-      have calls_to_prop (historyitem.nop :: rest) = calls_to_prop rest, by unfold calls_to_prop,
-      show ¬ free_in_prop x (historyitem.nop :: rest), from this.symm ▸ h2
-    )
-    ( -- <call> :: rest
-      assume f x' R S e σ vₓ,
-      assume x_free: free_in_prop x (calls_to_prop (call f x' R S e σ vₓ :: rest)),
-      have calls_to_prop (call f x' R S e σ vₓ :: rest) =
-        (prop.call (value.func f x' R S e σ) vₓ ⋀ calls_to_prop rest), by unfold calls_to_prop,
-      have x_free_in_prop: free_in_prop x (
-        prop.call (value.func f x' R S e σ) vₓ ⋀
-        calls_to_prop rest), from this ▸ x_free,
-      have x_not_free_in_vₓ: ¬ free_in_term x vₓ, from (
-        assume x_free_in_vₓ: free_in_term x vₓ,
-        show «false», by cases x_free_in_vₓ
+lemma call_history_closed (H: history) (x: var): ¬ free_in_prop x (calls_to_prop H) :=
+  begin
+    induction H with H₁ f y R S e H₂ σ v ih₁ ih₂,
+
+    show ¬free_in_prop x (calls_to_prop history.empty), from (
+      assume x_free: free_in_prop x (calls_to_prop history.empty),
+      have calls_to_prop history.empty = value.true, from rfl,
+      have x_free_in_true: free_in_prop x value.true, from this ▸ x_free,
+      show «false», by begin
+        cases x_free_in_true,
+        case free_in_prop.term x_free_in_term {
+          cases x_free_in_term
+        }
+      end
+    ),
+
+    show ¬free_in_prop x (calls_to_prop (H₁ · call f y R S e H₂ σ v)), from (
+      assume x_free: free_in_prop x (calls_to_prop (H₁ · call f y R S e H₂ σ v)),
+      have calls_to_prop (H₁ · call f y R S e H₂ σ v) =
+        (calls_to_prop H₁ ⋀ prop.call (value.func f y R S e H₂ σ) v), by unfold calls_to_prop,
+      have x_free_in_prop: free_in_prop x (calls_to_prop H₁ ⋀
+        prop.call (value.func f y R S e H₂ σ) v), from this ▸ x_free,
+      have x_not_free_in_v: ¬ free_in_term x v, from (
+        assume x_free_in_v: free_in_term x v,
+        show «false», by cases x_free_in_v
       ),
-      have x_not_free_in_f: ¬ free_in_term x (value.func f x' R S e σ), from (
-        assume x_free_in_f: free_in_term x (value.func f x' R S e σ),
+      have x_not_free_in_f: ¬ free_in_term x (value.func f y R S e H₂ σ), from (
+        assume x_free_in_f: free_in_term x (value.func f y R S e H₂ σ),
         show «false», by cases x_free_in_f
       ),
       have
-        free_in_prop x (calls_to_prop rest) ∨
-        free_in_prop x (prop.call (value.func f x' R S e σ) vₓ),
-      from (free_in_prop.and.inv x_free_in_prop).symm,
-      or.elim this ih (
-        assume x_free_in_call: free_in_prop x (prop.call (value.func f x' R S e σ) vₓ),
+        free_in_prop x (calls_to_prop H₁) ∨
+        free_in_prop x (prop.call (value.func f y R S e H₂ σ) v),
+      from (free_in_prop.and.inv x_free_in_prop),
+      or.elim this ih₁ (
+        assume x_free_in_call: free_in_prop x (prop.call (value.func f y R S e H₂ σ) v),
         show «false», by begin
           cases x_free_in_call,
           case free_in_prop.call₁ x_free_in_f {
             show «false», from x_not_free_in_f x_free_in_f
           },
-          case free_in_prop.call₂ x_free_in_vₓ {
-            show «false», from x_not_free_in_vₓ x_free_in_vₓ
+          case free_in_prop.call₂ x_free_in_v {
+            show «false», from x_not_free_in_v x_free_in_v
           }
         end
       )
     )
-  )
+  end
 
 lemma env.contains.inv {σ: env} {x y: var} {v: value}: x ∈ (σ[y↦v]) → (x = y ∨ x ∈ σ) :=
   assume x_in: x ∈ (σ[y↦v]),
@@ -476,7 +467,7 @@ lemma env.contains.same.inv {σ: env} {x y: var} {v: value}: x ∉ (σ[y↦v]) �
 lemma env.contains_apply_equiv {σ: env} {x: var}:
   ((σ x = none) ↔ (x ∉ σ)) ∧ ((∃v, σ x = some v) ↔ (x ∈ σ)) :=
 begin
-  induction σ with y v' σ' ih,
+  induction σ with σ' y v' ih,
   show ((env.empty x = none) ↔ (x ∉ env.empty)) ∧ ((∃v, env.empty x = some v) ↔ (x ∈ env.empty)), by begin
     split,
     show (env.empty x = none) ↔ (x ∉ env.empty), by begin
